Foundation/Modal/Kripke/Hilbert/GL/Soundness.lean
@@ -12,10 +12,10 @@ open Kripke
 
 namespace Kripke
 
-instance : TransitiveIrreflexiveFiniteFrameClass.DefinedBy {Axioms.K (atom 0) (atom 1), Axioms.L (atom 0)} :=
+instance : FrameClass.finite_transitive_irreflexive.DefinedBy {Axioms.K (atom 0) (atom 1), Axioms.L (atom 0)} :=
   FiniteFrameClass.definedBy_with_axiomK TransitiveIrreflexiveFiniteFrameClass.DefinedByL
 
-instance : TransitiveIrreflexiveFiniteFrameClass.IsNonempty := by
+instance : FrameClass.finite_transitive_irreflexive.IsNonempty := by
   use ⟨Unit, λ _ _ => False⟩;
   simp [Irreflexive , Transitive];
 
@@ -24,10 +24,10 @@ end Kripke
 
 namespace Hilbert.GL
 
-instance Kripke.finiteSound : Sound (Hilbert.GL) TransitiveIrreflexiveFiniteFrameClass := inferInstance
+instance Kripke.finiteSound : Sound (Hilbert.GL) FrameClass.finite_transitive_irreflexive := inferInstance
 
 instance Kripke.consistent : Entailment.Consistent (Hilbert.GL) :=
-  Kripke.Hilbert.consistent_of_FiniteFrameClass TransitiveIrreflexiveFiniteFrameClass
+  Kripke.Hilbert.consistent_of_FiniteFrameClass FrameClass.finite_transitive_irreflexive
 
 end Hilbert.GL
 
