Foundation/Modal/Kripke/Hilbert/K.lean
@@ -2,7 +2,6 @@ import Foundation.Modal.Hilbert.K
 import Foundation.Modal.Kripke.Hilbert.Soundness
 import Foundation.Modal.Kripke.Completeness
 import Foundation.Modal.Kripke.Filteration
-import Foundation.Modal.Kripke.FiniteFrame
 
 namespace LO.Modal
 
@@ -10,29 +9,26 @@ open Kripke
 
 namespace Hilbert.K
 
-instance Kripke.sound : Sound (Hilbert.K) AllFrameClass := inferInstance
+instance Kripke.sound : Sound (Hilbert.K) FrameClass.all := inferInstance
 
-instance : Entailment.Consistent (Hilbert.K) := Hilbert.consistent_of_FrameClass AllFrameClass
+instance : Entailment.Consistent (Hilbert.K) := Hilbert.consistent_of_FrameClass FrameClass.all (by simp)
 
-instance : Kripke.Canonical (Hilbert.K) (AllFrameClass) := ⟨by trivial⟩
+instance : Kripke.Canonical (Hilbert.K) FrameClass.all := ⟨by trivial⟩
 
-instance Kripke.completeAll : Complete (Hilbert.K) (AllFrameClass) := inferInstance
+instance Kripke.complete : Complete (Hilbert.K) FrameClass.all := inferInstance
 
-instance Kripke.completeAllFinite : Complete (Hilbert.K) (AllFiniteFrameClass) := ⟨by
+instance Kripke.complete_finiteAux : Complete (Hilbert.K) (FiniteFrameClass.all) := ⟨by
   intro φ hp;
-  apply Kripke.completeAll.complete;
+  apply Kripke.complete.complete;
   intro F _ V x;
   let M : Kripke.Model := ⟨F, V⟩;
   let FM := coarsestFilterationModel M ↑φ.subformulas;
 
   apply filteration FM (coarsestFilterationModel.filterOf) (by aesop) |>.mpr;
-  apply hp (by
-    suffices Finite (FilterEqvQuotient M φ.subformulas) by
-      use ⟨FM.toFrame⟩;
-      simp [FiniteFrameClass.toFrameClass];
-    apply FilterEqvQuotient.finite;
+  apply validOnModel_of_validOnFiniteFrameClass hp;
+  . tauto;
+  . apply FilterEqvQuotient.finite;
     simp;
-  ) FM.Val
 ⟩
 
 end Hilbert.K
