Foundation/Modal/Kripke/Hilbert/KTB.lean
@@ -1,53 +1,46 @@
 import Foundation.Modal.Kripke.Hilbert.Geach
 import Foundation.Modal.Kripke.Filteration
-import Foundation.Modal.Kripke.FiniteFrame
 
 namespace LO.Modal
 
 open Kripke
 open Geachean
 
-abbrev Kripke.ReflexiveSymmetricFrameClass : FrameClass := { F | Reflexive F ∧ Symmetric F }
-abbrev Kripke.ReflexiveSymmetricFiniteFrameClass : FiniteFrameClass := { F | Reflexive F.Rel ∧ Symmetric F.Rel }
+abbrev Kripke.FrameClass.refl_symm : FrameClass := { F | Reflexive F ∧ Symmetric F }
+abbrev Kripke.FiniteFrameClass.refl_symm : FiniteFrameClass := { F | Reflexive F.Rel ∧ Symmetric F.Rel }
 
-namespace Hilbert.KTB
+namespace Hilbert.KTB.Kripke
 
-instance Kripke.sound : Sound (Hilbert.KTB) (Kripke.ReflexiveSymmetricFrameClass) := by
+instance sound : Sound (Hilbert.KTB) Kripke.FrameClass.refl_symm := by
   convert Hilbert.Geach.Kripke.sound (G := {⟨0, 0, 1, 0⟩, ⟨0, 1, 0, 1⟩});
   . exact eq_Geach;
-  . unfold ReflexiveSymmetricFrameClass MultiGeacheanConfluentFrameClass MultiGeachean;
+  . unfold Kripke.FrameClass.refl_symm FrameClass.multiGeachean MultiGeachean;
     simp [Geachean.reflexive_def, Geachean.symmetric_def];
 
-instance Kripke.consistent : Entailment.Consistent (Hilbert.KTB) := by
-  convert Hilbert.Geach.Kripke.Consistent (G := {⟨0, 0, 1, 0⟩, ⟨0, 1, 0, 1⟩});
+instance consistent : Entailment.Consistent (Hilbert.KTB) := by
+  convert Hilbert.Geach.Kripke.consistent (G := {⟨0, 0, 1, 0⟩, ⟨0, 1, 0, 1⟩});
   exact eq_Geach;
 
-instance Kripke.canonical : Canonical (Hilbert.KTB) (ReflexiveSymmetricFrameClass) := ⟨⟨Canonical.reflexive, Canonical.symmetric⟩⟩
+instance canonical : Canonical (Hilbert.KTB) Kripke.FrameClass.refl_symm := ⟨⟨Canonical.reflexive, Canonical.symmetric⟩⟩
 
-instance Kripke.complete : Complete (Hilbert.KTB) (ReflexiveSymmetricFrameClass) := inferInstance
+instance complete : Complete (Hilbert.KTB) Kripke.FrameClass.refl_symm := inferInstance
 
-instance Kripke.finiteComplete : Complete (Hilbert.KTB) (ReflexiveSymmetricFiniteFrameClass) := ⟨by
+instance finite_complete : Complete (Hilbert.KTB) Kripke.FiniteFrameClass.refl_symm := ⟨by
   intro φ hp;
   apply Kripke.complete.complete;
   intro F ⟨F_refl, F_symm⟩ V x;
   let M : Kripke.Model := ⟨F, V⟩;
   let FM := finestFilterationModel M φ.subformulas;
   apply filteration FM (finestFilterationModel.filterOf) (by aesop) |>.mpr;
-  apply hp (by
-    suffices Finite (FilterEqvQuotient M φ.subformulas) by
-      simp only [FiniteFrameClass.toFrameClass, ReflexiveSymmetricFiniteFrameClass, Set.mem_image, Set.mem_setOf_eq];
-      use ⟨FM.toFrame⟩;
-      refine ⟨⟨?_, ?_⟩, ?_⟩;
-      . apply reflexive_filterOf_of_reflexive (finestFilterationModel.filterOf);
-        exact F_refl;
-      . apply finestFilterationModel.symmetric_of_symmetric;
-        exact F_symm;
-      . rfl;
-    apply FilterEqvQuotient.finite;
+  apply validOnModel_of_validOnFiniteFrameClass hp;
+  . refine ⟨?_, ?_⟩;
+    . apply reflexive_filterOf_of_reflexive (finestFilterationModel.filterOf);
+      exact F_refl;
+    . exact finestFilterationModel.symmetric_of_symmetric F_symm;;
+  . apply FilterEqvQuotient.finite;
     simp;
-  ) FM.Val
 ⟩
 
-end Hilbert.KTB
+end Hilbert.KTB.Kripke
 
 end LO.Modal
