Foundation/Modal/Kripke/Hilbert/KTc.lean
@@ -5,23 +5,23 @@ namespace LO.Modal
 open Kripke
 open Geachean
 
-abbrev Kripke.CoreflexiveFrameClass : FrameClass := { F | Coreflexive F }
+abbrev Kripke.FrameClass.corefl : FrameClass := { F | Coreflexive F }
 
 namespace Hilbert.KTc
 
-instance Kripke.sound : Sound (Hilbert.KTc) (Kripke.CoreflexiveFrameClass) := by
+instance Kripke.sound : Sound (Hilbert.KTc) Kripke.FrameClass.corefl := by
   convert Hilbert.Geach.Kripke.sound (G := {⟨0, 1, 0, 0⟩});
   exact eq_Geach;
-  . unfold CoreflexiveFrameClass MultiGeacheanConfluentFrameClass MultiGeachean;
+  . unfold Kripke.FrameClass.corefl FrameClass.multiGeachean MultiGeachean;
     simp [Geachean.reflexive_def, Geachean.coreflexive_def];
 
 instance Kripke.consistent : Entailment.Consistent (Hilbert.KTc) := by
-  convert Hilbert.Geach.Kripke.Consistent (G := {⟨0, 1, 0, 0⟩});
+  convert Hilbert.Geach.Kripke.consistent (G := {⟨0, 1, 0, 0⟩});
   exact eq_Geach;
 
-instance Kripke.canonical : Canonical (Hilbert.KTc) (CoreflexiveFrameClass) := ⟨Canonical.coreflexive⟩
+instance Kripke.canonical : Canonical (Hilbert.KTc) Kripke.FrameClass.corefl := ⟨Canonical.coreflexive⟩
 
-instance Kripke.complete : Complete (Hilbert.KTc) (CoreflexiveFrameClass) := inferInstance
+instance Kripke.complete : Complete (Hilbert.KTc) Kripke.FrameClass.corefl := inferInstance
 
 end Hilbert.KTc
 
