Foundation/Modal/Kripke/Hilbert/Soundness.lean
@@ -1,10 +1,10 @@
 import Foundation.Modal.Hilbert.Basic
-import Foundation.Modal.Kripke.FiniteFrame
+import Foundation.Modal.Kripke.Basic
 
 namespace LO.Modal
 
-open Kripke
 open Formula
+open Kripke
 open Formula.Kripke
 
 namespace Kripke.Hilbert
@@ -50,75 +50,23 @@ instance [defs : C.DefinedBy H.axioms] : C.DefinedBy H.axiomInstances := ⟨by
 
 instance [C.DefinedBy H.axioms] : Sound H C := ⟨fun {_} => soundness_of_FrameClass_definedBy_axiomInstances⟩
 
-lemma consistent_of_FrameClass_aux [nonempty : C.IsNonempty] [sound : Sound H C] : H ⊬ ⊥ := by
+lemma consistent_of_FrameClass (C : Kripke.FrameClass) (C_nonempty: C.Nonempty := by simp) [sound : Sound H C] : Entailment.Consistent H := by
+  apply Entailment.Consistent.of_unprovable (f := ⊥);
   apply not_imp_not.mpr sound.sound;
-  apply ValidOnFrameClass.not_of_exists_frame;
-  obtain ⟨F, hF⟩ := nonempty;
+  apply Semantics.set_models_iff.not.mpr;
+  push_neg;
+  obtain ⟨F, hF⟩ := C_nonempty;
   use F;
   constructor;
   . assumption;
   . simp;
 
-lemma consistent_of_FrameClass (C : Kripke.FrameClass) [C.IsNonempty] [Sound H C] : Entailment.Consistent H := by
-  apply Entailment.Consistent.of_unprovable;
-  exact consistent_of_FrameClass_aux (C := C);
-
-end
-
-
-section
-
-variable {C : Kripke.FiniteFrameClass}
-
-lemma soundness_of_FiniteFrameClass_definedBy_axiomInstances [defined : C.DefinedBy H.axiomInstances] : H ⊢! φ → C ⊧ φ := by
-  rintro hφ _ ⟨F, ⟨hF, rfl⟩⟩;
-  induction hφ using Hilbert.Deduction.rec! with
-  | maxm h =>
-    obtain ⟨ψ, h, ⟨s, rfl⟩⟩ := h;
-    apply defined.defines F |>.mp hF (ψ⟦s⟧);
-    use ψ;
-    constructor;
-    . assumption;
-    . use s;
-  | mdp ihpq ihp => exact ValidOnFrame.mdp ihpq ihp;
-  | nec ih => exact ValidOnFrame.nec ih;
-  | imply₁ => exact ValidOnFrame.imply₁;
-  | imply₂ => exact ValidOnFrame.imply₂;
-  | ec => exact ValidOnFrame.elimContra;
-
-instance [defs : C.DefinedBy H.axioms] : C.DefinedBy H.axiomInstances := ⟨by
-  intro F;
-  constructor;
-  . rintro hF φ ⟨ψ, hψ, ⟨s, rfl⟩⟩;
-    exact ValidOnFrame.subst $ defs.defines F |>.mp hF ψ hψ;
-  . intro h;
-    apply defs.defines F |>.mpr;
-    intro φ hφ;
-    apply h;
-    use φ;
-    constructor;
-    . assumption;
-    . use .id;
-      simp;
+lemma finite_sound_of_sound (sound : Sound H C) : Sound H ({ F | F ∈ C ∧ Finite F }) := ⟨by
+  rintro φ hφ F ⟨hF₁, _⟩;
+  exact sound.sound hφ hF₁;
 ⟩
 
-instance [C.DefinedBy H.axioms] : Sound H C := ⟨fun {_} => soundness_of_FiniteFrameClass_definedBy_axiomInstances⟩
-
-lemma consistent_of_FiniteFrameClass_aux [nonempty : C.IsNonempty] [sound : Sound H C] : H ⊬ ⊥ := by
-  apply not_imp_not.mpr sound.sound;
-  apply ValidOnFrameClass.not_of_exists_frame;
-  obtain ⟨F, hF⟩ := nonempty;
-  use F.toFrame;
-  constructor;
-  . use F;
-  . simp;
-
-lemma consistent_of_FiniteFrameClass (C : Kripke.FiniteFrameClass) [C.IsNonempty] [Sound H C] : Entailment.Consistent H := by
-  apply Entailment.Consistent.of_unprovable;
-  exact consistent_of_FiniteFrameClass_aux (C := C);
-
 end
-
 
 end Kripke.Hilbert
 
