Foundation/Modal/Logic/Sublogic/Grz.lean
@@ -9,7 +9,7 @@ open Kripke
 theorem S4_ssubset_Grz : Logic.S4 ⊂ Logic.Grz := by
   constructor;
   . exact Hilbert.weakerThan_of_dominate_axioms (by simp) |>.subset;
-  . suffices ∃ φ, Hilbert.Grz ⊢! φ ∧ ¬ReflexiveTransitiveFrameClass ⊧ φ by simpa [S4.eq_ReflexiveTransitiveKripkeFrameClass_Logic];
+  . suffices ∃ φ, Hilbert.Grz ⊢! φ ∧ ¬Kripke.FrameClass.preorder ⊧ φ by simpa [S4.eq_ReflexiveTransitiveKripkeFrameClass_Logic];
     use Axioms.Grz (.atom 0)
     constructor;
     . exact axiomGrz!;
