Foundation/Modal/ModalCompanion/LC.lean
@@ -74,7 +74,7 @@ instance modalCompanion_LC_S4Point3 : ModalCompanion Logic.LC Logic.S4Point3 := 
   rw [Logic.S4Point3.is_smallestMC_of_LC];
   exact Modal.instModalCompanion_of_smallestMC_via_KripkeSemantics
     (IC := Kripke.FrameClass.connected)
-    (MC := Modal.Kripke.ReflexiveTransitiveConnectedFrameClass)
+    (MC := Kripke.connected_preorder)
     (by
       intro φ;
       constructor;
